src/Utils/EGraph/QueryOpt.v
@@ -137,10 +137,10 @@ Section WithMap.
   #[local] Instance map_default {K V} `{m : map.map K V} : WithDefault m := map.empty.
 
   Definition remove_atom a {A} : state (instance A) unit :=
-    fun '(Build_instance _ _ _ _ _ _ db equiv parents epoch wl an) =>
+    fun '(Build_instance _ _ _ _ _ _ db equiv parents epoch wl an log) =>
       let tbl_upd tbl := map.remove tbl a.(atom_args) in
       let db' := map_update db a.(atom_fn) tbl_upd in
-      (tt,Build_instance _ _ _ _ _ _ db' equiv parents epoch wl an).
+      (tt,Build_instance _ _ _ _ _ _ db' equiv parents epoch wl an log).
 
   (*TODO: would this be a better signature for UnionFind.find? *)
   Definition uf_find_stateful i : state (union_find idx (idx_map idx) (idx_map nat)) idx :=
@@ -153,9 +153,9 @@ Section WithMap.
     list_Miter uf_find_stateful (map.keys uf.(parent _ _ _)) uf.
     
   Definition force_equiv {X} : state (instance X) unit :=
-    fun '(Build_instance _ _ _ _ _ _ db equiv parents epoch wl an) =>
+    fun '(Build_instance _ _ _ _ _ _ db equiv parents epoch wl an log) =>
       let equiv' := snd (force_uf equiv) in
-      (tt,Build_instance _ _ _ _ _ _ db equiv' parents epoch wl an).
+      (tt,Build_instance _ _ _ _ _ _ db equiv' parents epoch wl an log).
 
   (*TODO: move to utils*)
   Ltac get_goal :=
@@ -454,9 +454,10 @@ Section SequentOfStates.
   Definition sequent_of_states := 
     Build_sequent _ _ (map atom_clause assumption_atoms)
       (map (uncurry eq_clause) conclusion_eqs_final++(map atom_clause conclusion_atoms)).
-
+(*
   Notation state_sound_for_model :=
     (state_sound_for_model _ idx_succ _ _ _ _ _).
+*)
 
   (*TODO: move to base utils*)
       Ltac inst_implication H :=
